

CSCA67: Assignment #1

Due on September 28, 2025 at 11:59pm

Professor Anya Tafliovich Ch. 1

Gosha Polstvin

Algebraic proofs for Question 1

1. $(a \rightarrow b) \wedge (b \rightarrow c)$ **vs.** $a \rightarrow c$

$$\begin{aligned}(a \rightarrow b) \wedge (b \rightarrow c) &\equiv (\neg a \vee b) \wedge (\neg b \vee c) \\ &\Rightarrow \neg a \vee c \equiv a \rightarrow c.\end{aligned}$$

Failure of converse. Take $(a, b, c) = (F, T, F)$. Then $a \rightarrow c = T$, but $(a \rightarrow b) \wedge (b \rightarrow c) = F$, so $a \rightarrow c$ does not imply $(a \rightarrow b) \wedge (b \rightarrow c)$.

2. $a \wedge (a \rightarrow b)$ **vs.** $a \rightarrow b$

$$a \wedge (a \rightarrow b) \Rightarrow a \rightarrow b,$$

since $a \rightarrow b$ is a conjunct of the left-hand formula.

Failure of converse. Take $(a, b) = (F, F)$. Then $a \rightarrow b = T$ but $a \wedge (a \rightarrow b) = F$, so $a \rightarrow b$ does not imply $a \wedge (a \rightarrow b)$.

3. $(a \rightarrow b) \wedge (a \rightarrow c)$ **vs.** $a \rightarrow (b \wedge c)$

$$\begin{aligned}(a \rightarrow b) \wedge (a \rightarrow c) &\equiv (\neg a \vee b) \wedge (\neg a \vee c) \\ &\equiv \neg a \vee (b \wedge c) \equiv a \rightarrow (b \wedge c),\end{aligned}$$

so the formulas are equivalent.

4. $(a \rightarrow c) \wedge (b \rightarrow c)$ **vs.** $(a \vee b) \rightarrow c$

$$\begin{aligned}(a \rightarrow c) \wedge (b \rightarrow c) &\equiv (\neg a \vee c) \wedge (\neg b \vee c) \\ &\equiv (\neg a \wedge \neg b) \vee c \equiv \neg(a \vee b) \vee c \equiv (a \vee b) \rightarrow c,\end{aligned}$$

so they are equivalent.

5. $a \leftrightarrow b$ **vs.** $(a \wedge b) \vee (\neg a \wedge \neg b)$

By definition of biconditional:

$$a \leftrightarrow b \equiv (a \wedge b) \vee (\neg a \wedge \neg b),$$

so the formulas are identical.

6. $a \rightarrow (b \rightarrow (c \rightarrow d))$ **vs.** $((a \wedge b) \wedge c) \rightarrow d$

$$\begin{aligned}a \rightarrow (b \rightarrow (c \rightarrow d)) &\equiv \neg a \vee (\neg b \vee (\neg c \vee d)) \\ &\equiv \neg(a \wedge b \wedge c) \vee d \equiv ((a \wedge b) \wedge c) \rightarrow d,\end{aligned}$$

so they are equivalent.

7. $(a \rightarrow b) \vee (b \rightarrow a)$ **vs.** $a \leftrightarrow b$

Left-hand side is a tautology:

$$\begin{aligned}(a \rightarrow b) \vee (b \rightarrow a) &\equiv (\neg a \vee b) \vee (\neg b \vee a) \\ &\equiv (\neg a \vee a) \vee (\neg b \vee b) \equiv \top.\end{aligned}$$

Right-hand side is not a tautology. Example: $(a, b) = (T, F)$ gives $a \leftrightarrow b = F$. Hence they are not equivalent.

8. $a \leftrightarrow b$ **vs.** $\neg a \leftrightarrow \neg b$

$$\begin{aligned}\neg a \leftrightarrow \neg b &\equiv (\neg a \wedge \neg b) \vee (a \wedge b) \\ &\equiv (a \wedge b) \vee (\neg a \wedge \neg b) \equiv a \leftrightarrow b,\end{aligned}$$

so they are equivalent.

9. $(a \wedge b) \rightarrow (c \wedge d)$ **vs.** $((a \rightarrow c) \wedge (a \rightarrow d)) \wedge ((b \rightarrow c) \wedge (b \rightarrow d))$

RHS implies LHS:

$$\begin{aligned}\text{RHS} &\equiv (\neg a \vee c) \wedge (\neg a \vee d) \wedge (\neg b \vee c) \wedge (\neg b \vee d) \\ &\equiv ((\neg a \vee c) \wedge (\neg b \vee c)) \wedge ((\neg a \vee d) \wedge (\neg b \vee d)) \\ &\equiv ((\neg a \wedge \neg b) \vee c) \wedge ((\neg a \wedge \neg b) \vee d) \\ &\equiv (\neg a \wedge \neg b) \vee (c \wedge d) \equiv (a \wedge b) \rightarrow (c \wedge d).\end{aligned}$$

Failure of converse. Example: $(a, b, c, d) = (T, F, F, F)$ gives LHS true, RHS false.

10. $(a \vee b) \rightarrow (c \wedge d)$ **vs.** $((a \rightarrow c) \wedge (a \rightarrow d)) \wedge ((b \rightarrow c) \wedge (b \rightarrow d))$

$$\begin{aligned}(a \vee b) \rightarrow (c \wedge d) &\equiv (\neg a \wedge \neg b) \vee (c \wedge d), \\ \text{RHS} &\equiv (\neg a \vee c) \wedge (\neg a \vee d) \wedge (\neg b \vee c) \wedge (\neg b \vee d) \\ &\equiv ((\neg a \vee c) \wedge (\neg b \vee c)) \wedge ((\neg a \vee d) \wedge (\neg b \vee d)) \\ &\equiv ((\neg a \wedge \neg b) \vee c) \wedge ((\neg a \wedge \neg b) \vee d) \\ &\equiv (\neg a \wedge \neg b) \vee (c \wedge d) \equiv (a \vee b) \rightarrow (c \wedge d),\end{aligned}$$

so they are equivalent.

Question 2. Tautology / contradiction / neither

We classify each formula and give succinct rigorous arguments.

1. $(a \rightarrow b) \vee (b \rightarrow a)$.

Classification: *Tautology*.

Proof. As in Question 1.7,

$$(\neg a \vee b) \vee (\neg b \vee a) \equiv (\neg a \vee a) \vee (\neg b \vee b) \equiv \top,$$

so the formula is true under every valuation. □

2. $((a \rightarrow b) \wedge (b \rightarrow c)) \wedge a \wedge \neg c.$

Classification: *Contradiction* (unsatisfiable).

Proof. Assume the whole conjunction is true. Then from $(a \rightarrow b) \wedge (b \rightarrow c)$ and a we can derive b and then c by successive modus ponens. But the formula also contains $\neg c$ as a conjunct, hence we deduce both c and $\neg c$, contradiction. Therefore there is no valuation that makes the formula true; it is a contradiction. \square

3. $((a \rightarrow b) \wedge (b \rightarrow c)) \wedge a \wedge c.$

Classification: *Neither* (satisfiable but not a tautology).

Proof. Satisfiable: take $a = b = c = T$. Then each of $a \rightarrow b$, $b \rightarrow c$ is T , and $a \wedge c$ is T , so the whole conjunction is T . Not a tautology: take $a = F, b = F, c = F$. Then the conjunct a is F , so the whole conjunction is F . Hence neither a tautology nor a contradiction. \square

4. $a \rightarrow \neg a.$

Classification: *Neither*.

Proof. If $a = F$ the implication $a \rightarrow \neg a$ is T (antecedent false). If $a = T$ the implication is $T \rightarrow F = F$. Thus the formula is satisfiable but not always true; hence neither. \square

5. $(a \wedge (a \rightarrow b)) \rightarrow b.$

Classification: *Tautology*.

Proof. Suppose $a \wedge (a \rightarrow b)$ holds. Then a holds and $a \rightarrow b$ holds, so by modus ponens b holds. Therefore the implication from $a \wedge (a \rightarrow b)$ to b is always true, i.e. a tautology. Algebraically one can expand the antecedent as $a \wedge (\neg a \vee b)$ and simplify to see the implication is always true, but the straightforward rule-based derivation via modus ponens is immediate and rigorous. \square

Question 3. Deductive reasoning (validity / proofs)

For each argument we indicate validity. If valid, we present (i) a truth-table style check covering all rows where the premises are all true, and (ii) a rules-of-inference (natural deduction) proof. If invalid, we give an explicit counterexample valuation.

(A) Truth Table

1. If the weather is good, I either go running or swimming. $W \rightarrow (R \vee S).$
2. I don't go running and swimming at the same time. $\neg(R \wedge S).$

Validity: *Valid*.

- | | |
|-------------------------------|---------|
| 1. $W \rightarrow (R \vee S)$ | Premise |
| 2. $\neg(R \wedge S)$ | Premise |

3. From $\neg(R \wedge S)$ we get $R \rightarrow \neg S$ and $S \rightarrow \neg R$. (Equivalently: $\neg(R \wedge S) \equiv \neg R \vee \neg S$, from which each implication follows; or prove each implication by conditional proof.)
4. To prove $(W \wedge R) \rightarrow \neg S$: assume $W \wedge R$.
 - (a) From $W \wedge R$ infer W and R .
 - (b) From W and $W \rightarrow (R \vee S)$ infer $R \vee S$.
 - (c) From R and $R \rightarrow \neg S$ infer $\neg S$.

Discharging the assumption $W \wedge R$ yields $(W \wedge R) \rightarrow \neg S$.

5. The proof of $(W \wedge S) \rightarrow \neg R$ is symmetric.

| R | S | W | $W \rightarrow (R \vee S)$ | $\neg(R \wedge S)$ | All Premises? | $(W \wedge R) \rightarrow \neg S$ | $(W \wedge S) \rightarrow \neg R$ |
|---|---|---|----------------------------|--------------------|---------------|-----------------------------------|-----------------------------------|
| F | F | F | T | T | T | T | T |
| F | F | T | F | T | F | T | T |
| F | T | F | T | T | T | T | T |
| F | T | T | T | T | T | T | T |
| T | F | F | T | T | T | T | T |
| T | F | T | T | T | T | T | T |
| T | T | F | T | F | F | T | T |
| T | T | T | T | F | F | T | T |

(B) Truth Table

Informal argument.

1. To get a good grade G it is necessary to attend lectures and do readings: $G \rightarrow (L \wedge R)$.
2. I attend lectures and do readings: $L \wedge R$.

Conclusion: G . **Validity:** *Invalid*.

Counterexample. Take the valuation $G = F$, $L = T$, $R = T$. Then $G \rightarrow (L \wedge R)$ is true (antecedent false) and $L \wedge R$ is true, but G is false. Therefore the premises can all be true while the conclusion is false; hence the argument is invalid. Intuitively the premise states “ $L \wedge R$ is *necessary* for G ”, which does not imply $L \wedge R$ is sufficient for G . \square

| G | L | R | $G \rightarrow (L \wedge R)$ | $L \wedge R$ | All Premises? | G |
|---|---|---|------------------------------|--------------|---------------|---|
| F | F | F | T | F | F | F |
| F | F | T | T | F | F | F |
| F | T | F | T | F | F | F |
| F | T | T | T | T | T | F |
| T | F | F | F | F | F | T |
| T | F | T | F | F | F | T |
| T | T | F | F | F | F | T |
| T | T | T | T | T | T | T |

(C) Truth Table

Informal argument.

1. $((L \wedge R \wedge E) \vee K) \rightarrow G$.
2. L, R, E .

Conclusion: G .

Validity: *Valid*.

- | | |
|---|------------------------|
| 1. $((L \wedge R \wedge E) \vee K) \rightarrow G$ | Premise |
| 2. L | Premise |
| 3. R | Premise |
| 4. E | Premise |
| 5. From 2–4 infer $L \wedge R \wedge E$. | \wedge -Introduction |
| 6. From 5 infer $(L \wedge R \wedge E) \vee K$. | \vee -Introduction |
| 7. From 1 and 6 infer G . | Modus Ponens |

Thus G follows; the argument is valid.

| L | R | E | K | G | $(L \wedge R \wedge E) \vee K$ | Premise1: antecedent $\rightarrow G$ | All Premises? | G |
|---|---|---|---|---|--------------------------------|--------------------------------------|---------------|---|
| F | F | F | F | F | F | T | F | F |
| F | F | F | F | T | F | T | F | T |
| F | F | F | T | F | T | F | F | F |
| F | F | F | T | T | T | T | F | T |
| F | F | T | F | F | F | T | F | F |
| F | F | T | F | T | F | T | F | T |
| F | F | T | T | F | T | F | F | F |
| F | F | T | T | T | T | T | F | T |
| F | T | F | F | F | F | T | F | F |
| F | T | F | F | T | F | T | F | T |
| F | T | F | T | F | T | F | F | F |
| F | T | F | T | T | T | T | F | T |
| F | T | T | F | F | F | T | F | F |
| F | T | T | F | T | F | T | F | T |
| F | T | T | T | F | T | F | F | F |
| F | T | T | T | T | T | T | F | T |
| T | F | F | F | F | F | T | F | F |
| T | F | F | F | T | F | T | F | T |
| T | F | F | T | F | T | F | F | F |
| T | F | F | T | T | T | T | F | T |
| T | F | T | F | F | F | T | F | F |
| T | F | T | F | T | F | T | F | T |
| T | F | T | T | F | T | F | F | F |
| T | F | T | T | T | T | T | F | T |
| T | T | F | F | F | F | T | F | F |
| T | T | F | F | T | F | T | F | T |
| T | T | F | T | F | T | F | F | F |
| T | T | F | T | T | T | T | F | T |
| T | T | T | F | F | T | F | F | F |
| T | T | T | F | T | T | T | T | T |
| T | T | T | T | F | T | F | F | F |
| T | T | T | T | T | T | T | T | T |

(D) Truth Table*Informal argument.*

1. $(L \rightarrow \neg B) \vee (K \rightarrow \neg C)$.
2. $B \vee C$.

Validity: *Invalid.**Counterexample.* Set

$$(B, C, L, K) = (T, F, T, T).$$

Evaluate:

$$L \rightarrow \neg B = T \rightarrow F = F, \quad K \rightarrow \neg C = T \rightarrow T = T,$$

so the disjunction $(L \rightarrow \neg B) \vee (K \rightarrow \neg C)$ is T. Also $B \vee C = T$. But the conclusion

$$\neg L \vee \neg K = \neg T \vee \neg T = F$$

is false. Therefore premises true and conclusion false, so the argument is invalid. \square

| L | K | B | C | $L \rightarrow \neg B$ | $K \rightarrow \neg C$ | $(L \rightarrow \neg B) \vee (K \rightarrow \neg C)$ | $B \vee C$ | $\neg L \vee \neg K$ |
|---|---|---|---|------------------------|------------------------|--|------------|----------------------|
| F | F | F | F | T | T | T | F | T |
| F | F | F | T | T | T | T | T | T |
| F | F | T | F | T | T | T | T | T |
| F | F | T | T | T | T | T | T | T |
| F | T | F | F | T | T | T | F | T |
| F | T | F | T | T | F | T | T | T |
| F | T | T | F | T | T | T | T | T |
| F | T | T | T | T | F | T | T | T |
| T | F | F | F | F | T | T | F | T |
| T | F | F | T | F | T | T | T | T |
| T | F | T | F | F | T | F | T | T |
| T | F | T | T | F | T | T | T | T |
| T | T | F | F | F | T | T | F | F |
| T | T | F | T | F | F | F | T | F |
| T | T | T | F | F | T | F | T | F |
| T | T | T | T | F | F | F | T | F |

(E) Truth Table

Informal argument.

1. $L \rightarrow \neg B$.
2. $K \rightarrow \neg C$.
3. $B \vee C$.

Conclusion: $\neg L \vee \neg K$. **Validity:** *Valid*.

- | | |
|--|---------|
| 1. $L \rightarrow \neg B$ | Premise |
| 2. $K \rightarrow \neg C$ | Premise |
| 3. $B \vee C$ | Premise |
| 4. Assume, for reductio, $L \wedge K$. | |
| (a) From assumption infer L and K . | |
| (b) From 1 and L infer $\neg B$. | |
| (c) From 2 and K infer $\neg C$. | |
| (d) From 3 and $\neg B, \neg C$ conclude contradiction, since $B \vee C$ together with $\neg B \wedge \neg C$ is impossible. | |
| 5. Hence $L \wedge K$ leads to contradiction; therefore $\neg(L \wedge K)$ holds. | |
| 6. By De Morgan, $\neg(L \wedge K) \equiv \neg L \vee \neg K$, which is the desired conclusion. | |

This completes the proof; the argument is valid.

| L | K | B | C | $L \rightarrow \neg B$ | $K \rightarrow \neg C$ | $B \vee C$ | $\neg L \vee \neg K$ |
|---|---|---|---|------------------------|------------------------|------------|----------------------|
| F | F | F | F | T | T | F | T |
| F | F | F | T | T | T | T | T |
| F | F | T | F | T | T | T | T |
| F | F | T | T | T | T | T | T |
| F | T | F | F | T | T | F | T |
| F | T | F | T | T | F | T | T |
| F | T | T | F | T | T | T | T |
| F | T | T | T | T | F | T | T |
| T | F | F | F | F | T | F | T |
| T | F | F | T | F | T | T | T |
| T | F | T | F | F | T | T | T |
| T | F | T | T | F | T | T | T |
| T | T | F | F | F | T | F | F |
| T | T | F | T | F | F | T | F |
| T | T | T | F | F | T | T | F |
| T | T | T | T | F | F | T | F |